\documentclass[12pt,twoside]{article}

\newcommand{\reporttitle}{477 - Computational Optimisation}
\newcommand{\reportauthor}{Jiahao Lin}
\newcommand{\reporttype}{Coursework}
\newcommand{\cid}{00837321}

% include files that load packages and define macros
\input{includes} % various packages needed for maths etc.
\input{notation} % short-hand notation and macros


%%%%%%%%%%%%%%%%%%%%%%%%%%%%

\begin{document}
% front page
\input{titlepage}


%%%%%%%%%%%%%%%%%%%%%%%%%%%% Main document
\section{Part 1}


\subsection{1}


\begin{enumerate}[1)]
\item 
To prove is $\log \sum_{k=1}^{10} exp(B_{jk})$ is convex, we define:
\begin{align}
f(B_j) = \log \sum_{k=1}^{10} exp(B_{jk})\\
f(x) = \log \sum_{k=1}^{10} exp(x_k)
\end{align}
First we need to compute the Hessian of $f(x)$:
\begin{align}
\nabla f(x) = \frac{1}{1\T Z} \times z\\
\nabla^2 f(x) = \frac{1}{1\T Z} \times diag(Z) - \frac{Z\T Z}{{(1\T Z)}^2}\\
where\quad Z = \sum_{k=1}^{10} exp(x_{k})
\end{align}
For convexity we need to prove the Hessian is positive semi-definite, we need to prove:
\begin{align}
\nabla^2 f(x) \succeq 0\\
v\T\nabla^2 f(x)v >= 0\\
v\T\left(\frac{1}{1\T Z} \times diag(Z) - \frac{Z\T Z}{{(1\T Z)}^2}\right)v >= 0\\
\frac{(\sum_{k=1}^{10} Z_k V_k^2) \sum_{k=1}^{10}Z_k - \sum_{k=1}^{10}(Z_k v_k)^2}{(1\T Z)^2} >=0
\end{align}
According to Cauchy-Schwartz inequality:
\begin{align}
\sum_{k=1}^{10}(Z_k v_k)^2 \leq \sum_{k=1}^{10}Z_k \times \sum_{k=1}^{10} (Z_k V_k^2)
\end{align}
There for the Hessian is positive semi-definite holds, the Log-Sum-Exp function is convex.
\item
Denote affine mapping on $\beta_k$ as $g(\beta_k)$:
\begin{align}
g(\beta_k) = x_i\T\beta_k
\end{align}
And denote Log-Sum-Exp function as $f(x_k)$:
\begin{align}
f(x_k) = \log \sum_{k=1}^{10} exp(x_{k})
\end{align}
Now we know that $f(x_k)$ is convex, and we want to prove that $f \circ g$ is convex as well, from the definition of convexity, we need to prove:
\begin{align}
f \circ g(\alpha x + (1-\alpha)y) \leq \alpha f \circ g(x) + (1-\alpha)f \circ g(y)\\
for \quad any \quad x,\quad y \quad and\quad  \alpha \in [0,1]
\end{align}
Since we know:
\begin{align}
g(\alpha x + (1-\alpha)y) = \alpha g(x) + (1-\alpha)g(y)
\end{align}
We can prove that:
\begin{align}
f \circ g(\alpha x + (1-\alpha)y) = f ( g(\alpha x + (1-\alpha)y))\\
= f ( \alpha g(x) + (1-\alpha)g(y))\\
\leq \alpha f \circ g(x) + (1-\alpha)f \circ g(y)
\end{align}
Now we know that $\log \sum_{k=1}^{10} exp(x_i\T \beta_k)$ is convex as well.
\item



\end{enumerate}





\end{document}
%%% Local Variables: 
%%% mode: latex
%%% TeX-master: t
%%% End: 
